More

Simple_Clause_Learning/Examples.thy
@@ -2,7 +2,7 @@ theory Examples
   imports Simple_Clause_Learning
 begin
 
-locale example = scl renaming_vars inv_renaming_vars
+(* locale example1 = scl renaming_vars inv_renaming_vars
   for renaming_vars inv_renaming_vars :: "'v set \<Rightarrow> 'v \<Rightarrow> 'v" +
   fixes a b c d e f g :: "('f, 'v) term"
   assumes distinct_terms: "distinct [a, b, c, d, e, f, g]" and
@@ -392,6 +392,602 @@ proof (unfold regular_scl_def, rule disjI1)
     apply simp
     apply (simp add: trail_false_cls_def trail_false_lit_def)
     oops
+
+end *)
+
+locale exampl2 = scl renaming_vars inv_renaming_vars
+  for renaming_vars inv_renaming_vars :: "'v set \<Rightarrow> 'v \<Rightarrow> 'v" +
+  fixes P Q R :: "('f, 'v) term"
+  assumes distinct_terms: "distinct [P, Q, R]" and
+    ball_is_ground_atm: "\<forall>t \<in> {P, Q, R}. is_ground_atm t"
+begin
+
+definition C1 :: "('f, 'v) term clause" where
+  "C1 = {#Pos P#}"
+
+definition C2 :: "('f, 'v) term clause" where
+  "C2 = {#Pos Q#}"
+
+definition C3 :: "('f, 'v) term clause" where
+  "C3 = {#Neg P, Pos R#}"
+
+definition C4 :: "('f, 'v) term clause" where
+  "C4 = {#Neg Q, Neg R#}"
+
+definition N :: "('f, 'v) term clause set" where
+  "N = {C1, C2, C3, C4}"
+
+lemma ball_is_ground_cls: "\<forall>C \<in> N. is_ground_cls C"
+  using ball_is_ground_atm
+  by (simp add: N_def C1_def C2_def C3_def C4_def is_ground_cls_def is_ground_lit_def)
+
+
+definition S1 where
+  "S1 = ([(Pos P, None)], {}, None)"
+
+lemma "regular_scl N initial_state S1"
+proof (unfold regular_scl_def, rule disjI2, rule conjI)
+  show "\<not> conflict N initial_state S1"
+    unfolding S1_def
+    by (simp add: conflict.simps)
+next
+  have "decide N initial_state (trail_decide [] (Pos P), {}, None)"
+    by (rule decideI)
+      (simp_all add: ball_is_ground_atm is_ground_lit_def trail_defined_lit_iff_true_or_false)
+  hence "scl N initial_state (trail_decide [] (Pos P), {}, None)"
+    by (simp add: scl_def)
+  moreover have "\<nexists>S. conflict N (trail_decide [] (Pos P), {}, None) S"
+    apply (rule notI)
+    apply (elim exE conflict.cases)
+    using ball_is_ground_cls distinct_terms
+    by (auto simp: N_def C1_def C2_def C3_def C4_def
+        trail_decide_def trail_false_cls_def trail_false_lit_def)
+  ultimately show "reasonable_scl N initial_state S1"
+    unfolding reasonable_scl_def by (simp add: S1_def trail_decide_def)
+qed
+
+
+definition S2 where
+  "S2 = ([
+    (Pos Q, None),
+    (Pos P, None)], {}, None)"
+
+lemma "regular_scl N S1 S2"
+proof (unfold regular_scl_def, rule disjI2, rule conjI)
+  show "\<not> conflict N S1 S2"
+    unfolding S1_def S2_def
+    by (simp add: conflict.simps)
+next
+  have "decide N S1 S2"
+    unfolding S1_def S2_def
+    using distinct_terms ball_is_ground_atm
+    by (auto simp: decide.simps trail_decide_def trail_defined_lit_def)
+  hence "scl N S1 S2"
+    unfolding scl_def by simp
+  moreover have "\<nexists>S. conflict N S2 S"
+    apply (rule notI)
+    apply (elim exE conflict.cases)
+    using ball_is_ground_cls distinct_terms
+    by (auto simp add: N_def S2_def C1_def C2_def C3_def C4_def trail_false_cls_def
+        trail_false_lit_def)
+  ultimately show "reasonable_scl N S1 S2"
+    unfolding reasonable_scl_def by simp
+qed
+
+
+definition S3 :: "('f, 'v) state" where
+  "S3 = ([
+    (Pos R, Some ({#Neg P#}, Pos R, Var)),
+    (Pos Q, None),
+    (Pos P, None)], {}, None)"
+
+lemma "scl N S2 S3"
+proof -
+  have "propagate N S2 S3"
+    unfolding S2_def S3_def
+    unfolding propagate.simps
+    apply (rule exI[of _ C3])
+    using distinct_terms ball_is_ground_cls ball_is_ground_atm
+    by (auto simp add: N_def C1_def C2_def C3_def trail_propagate_def is_ground_cls_def trail_false_cls_def
+        trail_false_lit_def trail_defined_lit_def)
+  thus "scl N S2 S3"
+    unfolding scl_def by simp
+qed
+
+
+definition S4 :: "('f, 'v) state" where
+  "S4 = ([
+    (Pos R, Some ({#Neg P#}, Pos R, Var)),
+    (Pos Q, None),
+    (Pos P, None)], {}, Some (C4, Var))"
+
+lemma "scl N S3 S4"
+proof -
+  have "conflict N S3 S4"
+    unfolding S3_def S4_def
+    unfolding conflict.simps
+    apply (rule exI[of _ C4])
+    using distinct_terms ball_is_ground_cls ball_is_ground_atm
+    by (simp add: N_def trail_false_cls_def C4_def trail_false_lit_def)
+  thus ?thesis
+    by (simp add: scl_def)
+qed
+
+
+definition S5 :: "('f, 'v) state" where
+  "S5 = ([
+    (Pos R, Some ({#Neg P#}, Pos R, Var)),
+    (Pos Q, None),
+    (Pos P, None)], {}, Some ({#Neg P, Neg Q#}, Var))"
+
+lemma "scl N S4 S5"
+proof -
+  have "resolve N S4 S5"
+    unfolding S4_def S5_def
+    unfolding resolve.simps
+    apply (rule exI[of _ "state_trail S4"])
+    apply (rule exI[of _ "tl (state_trail S4)"])
+    (* using S4_def C4_def *)
+    apply (rule exI[of _ "Pos R"])
+    apply (rule exI[of _ "{#Neg P#}"])
+    apply (rule exI[of _ Var])
+    apply (rule exI[of _ "renaming_wrt (N \<union> clss_of_trail (fst S4) \<union> {{#Neg Q#} + {#Neg P#}})"])
+    apply (rule exI[of _ "{}"])
+    apply (rule exI[of _ "{#Neg Q#}"])
+    apply (rule exI[of _ "Neg R"])
+    apply (rule exI[of _ Var])
+    apply (rule exI[of _ Var])
+    using distinct_terms ball_is_ground_cls ball_is_ground_atm
+    by (simp add: S4_def is_decision_lit_def C4_def trail_propagate_def trail_level_cls_def is_ground_atm_iff_vars_empty)
+  thus ?thesis
+    by (simp add: scl_def)
+qed
+
+lemma "grounding_of_clss N \<TTurnstile>e grounding_of_clss {{#Neg P, Neg Q#}}"
+proof -
+  have "is_ground_cls {#Neg P, Neg Q#}"
+    using ball_is_ground_cls
+    by (simp add: N_def C1_def C2_def is_ground_cls_def is_ground_lit_def)
+  hence "grounding_of_clss {{#Neg P, Neg Q#}} = {{#Neg P, Neg Q#}}"
+    by (simp add: grounding_of_cls_ground)
+
+  have "grounding_of_clss N = {C1, C2, C3, C4}"
+    using ball_is_ground_cls
+    unfolding N_def C1_def C2_def C3_def C4_def
+    by (auto simp add: grounding_of_clss_def grounding_of_cls_ground)
+
+  show ?thesis
+    unfolding \<open>grounding_of_clss N = {C1, C2, C3, C4}\<close>
+    unfolding \<open>grounding_of_clss {{#Neg P, Neg Q#}} = {{#Neg P, Neg Q#}}\<close>
+    unfolding C1_def C2_def C3_def C4_def
+  proof (intro allI impI)
+    fix I
+    assume "I \<TTurnstile>s {{#Pos P#}, {#Pos Q#}, {#Neg P, Pos R#}, {#Neg Q, Neg R#}}"
+    hence "P \<in> I \<and> Q \<in> I \<and> R \<in> I \<and> R \<notin> I"
+      by blast
+    hence False by simp
+    thus "I \<TTurnstile>s {{#Neg P, Neg Q#}}" by simp
+  qed
+qed
+
+
+definition S6 :: "('f, 'v) state" where
+  "S6 = ([
+    (Pos Q, None),
+    (Pos P, None)], {}, Some ({#Neg P, Neg Q#}, Var))"
+
+lemma "scl N S5 S6"
+proof -
+  have "skip N S5 S6"
+    unfolding S5_def S6_def skip.simps
+    using distinct_terms by (auto simp add: trail_propagate_def)
+  thus ?thesis
+    by (simp add: scl_def)
+qed
+
+lemma "\<nexists>S7. scl N S6 S7"
+proof (rule notI, unfold scl_def, elim exE disjE)
+  fix S7
+  show "propagate N S6 S7 \<Longrightarrow> False"
+    unfolding S6_def propagate.simps by simp
+next
+  fix S7
+  show "decide N S6 S7 \<Longrightarrow> False"
+    unfolding S6_def decide.simps by simp
+next
+  fix S7
+  show "conflict N S6 S7 \<Longrightarrow> False"
+    unfolding S6_def conflict.simps by simp
+next
+  fix S7
+  show "skip N S6 S7 \<Longrightarrow> False"
+    unfolding S6_def skip.simps by (simp add: trail_propagate_def)
+next
+  fix S7
+  show "factorize N S6 S7 \<Longrightarrow> False"
+    unfolding S6_def factorize.simps
+    using distinct_terms
+    apply (simp add: trail_propagate_def)
+    apply (elim exE)
+    by (metis (no_types, opaque_lifting) add_eq_conv_ex add_mset_eq_single literal.sel(2))
+next
+  fix S7
+  show "resolve N S6 S7 \<Longrightarrow> False"
+    unfolding S6_def resolve.simps by (simp add: trail_propagate_def)
+next
+  fix S7
+  show "backtrack N S6 S7 \<Longrightarrow> False"
+    oops
+
+end
+
+locale exampl3 = scl renaming_vars inv_renaming_vars
+  for renaming_vars inv_renaming_vars :: "'v set \<Rightarrow> 'v \<Rightarrow> 'v" +
+  fixes P Q R S :: 'f and v w x y z :: 'v and a b :: "('f, 'v) term"
+  assumes
+    distinct_preds: "distinct [P, Q, R, S]" and
+    distinct_vars: "distinct [v, w, x, y, z]" and
+    distinct_terms: "distinct [a, b]" and
+    ground_a[simp]: "is_ground_atm a" and
+    ground_b[simp]: "is_ground_atm b"
+begin
+
+lemma ground_Fun[simp]: "\<And>f a. is_ground_atm a \<Longrightarrow> is_ground_atm (Fun f [a])"
+  unfolding is_ground_atm_iff_vars_empty by simp
+
+definition N :: "('f, 'v) term clause set" where
+  "N = {
+    {#Pos (Fun P [Var x])#},
+    {#Pos (Fun Q [Var y])#},
+    {#Neg (Fun Q [Var z]), Pos (Fun R [Var z])#},
+    {#Neg (Fun R [Var w]), Pos (Fun S [Var w])#},
+    {#Neg (Fun P [Var v]), Neg (Fun S [Var v])#}}"
+
+definition S1 :: "('f, 'v) state"  where
+  "S1 = ([(Pos (Fun P [a]), None)], {}, None)"
+
+lemma "regular_scl N initial_state S1"
+proof (unfold regular_scl_def, rule disjI2, rule conjI)
+  show "\<not> conflict N initial_state S1"
+    unfolding S1_def
+    by (simp add: conflict.simps)
+next
+  have "decide N initial_state (trail_decide [] (Pos (Fun P [a])), {}, None)"
+    by (rule decideI) simp_all
+  hence "scl N initial_state S1"
+    by (simp add: S1_def scl_def trail_decide_def)
+  moreover have "\<nexists>S. conflict N S1 S"
+  proof (rule notI, erule exE)
+    fix S
+    assume "conflict N S1 S"
+    thus False
+      unfolding S1_def
+      apply (cases rule: conflict.cases)
+      unfolding N_def Un_empty_right insert_iff
+      apply (elim disjE)
+      using distinct_preds
+      by (simp_all add: rename_clause_def clss_of_trail_def trail_false_cls_def
+          trail_false_lit_def subst_lit_def)
+  qed
+  ultimately show "reasonable_scl N initial_state S1"
+    unfolding reasonable_scl_def by (simp add: S1_def)
+qed
+
+definition S2 :: "('f, 'v) state"  where
+  "S2 = ([
+    (Pos (Fun Q [a]), None),
+    (Pos (Fun P [a]), None)], {}, None)"
+
+lemma "regular_scl N S1 S2"
+proof (unfold regular_scl_def, rule disjI2, rule conjI)
+  show "\<not> conflict N S1 S2"
+    unfolding S1_def S2_def
+    by (simp add: conflict.simps)
+next
+  have "decide N S1 (trail_decide (state_trail S1) (Pos (Fun Q [a])), {}, None)"
+    unfolding S1_def state_trail_simp
+    using distinct_preds by (auto simp: trail_defined_lit_def intro: decideI)
+  hence "scl N S1 S2"
+    by (simp add: S1_def S2_def scl_def trail_decide_def)
+  moreover have "\<nexists>S. conflict N S2 S"
+  proof (rule notI, erule exE)
+    fix S
+    assume "conflict N S2 S"
+    thus False
+      unfolding S2_def
+      apply (cases rule: conflict.cases)
+      unfolding N_def Un_empty_right insert_iff
+      apply (elim disjE)
+      using distinct_preds
+      by (auto simp add: rename_clause_def clss_of_trail_def trail_false_cls_def
+          trail_false_lit_def subst_lit_def)
+  qed
+  ultimately show "reasonable_scl N S1 S2"
+    unfolding reasonable_scl_def by (simp add: S1_def)
+qed
+
+definition S3 :: "('f, 'v) state"  where
+  "S3 = ([
+    (Pos (Fun P [b]), None),
+    (Pos (Fun Q [a]), None),
+    (Pos (Fun P [a]), None)], {}, None)"
+
+lemma "regular_scl N S2 S3"
+proof (unfold regular_scl_def, rule disjI2, rule conjI)
+  show "\<not> conflict N S2 S3"
+    unfolding S2_def S3_def
+    by (simp add: conflict.simps)
+next
+  have "decide N S2 (trail_decide (state_trail S2) (Pos (Fun P [b])), {}, None)"
+    unfolding S2_def state_trail_simp
+    using distinct_preds distinct_terms by (auto simp: trail_defined_lit_def intro: decideI)
+  hence "scl N S2 S3"
+    by (simp add: S2_def S3_def scl_def trail_decide_def)
+  moreover have "\<nexists>S. conflict N S3 S"
+  proof (rule notI, erule exE)
+    fix S
+    assume "conflict N S3 S"
+    thus False
+      unfolding S3_def
+      apply (cases rule: conflict.cases)
+      unfolding N_def Un_empty_right insert_iff
+      apply (elim disjE)
+      using distinct_preds
+      by (auto simp add: rename_clause_def clss_of_trail_def trail_false_cls_def
+          trail_false_lit_def subst_lit_def)
+  qed
+  ultimately show "reasonable_scl N S2 S3"
+    unfolding reasonable_scl_def by (simp add: S1_def)
+qed
+
+definition S4 :: "('f, 'v) state"  where
+  "S4 = ([
+    (Pos (Fun Q [b]), None),
+    (Pos (Fun P [b]), None),
+    (Pos (Fun Q [a]), None),
+    (Pos (Fun P [a]), None)], {}, None)"
+
+lemma "regular_scl N S3 S4"
+proof (unfold regular_scl_def, rule disjI2, rule conjI)
+  show "\<not> conflict N S3 S4"
+    unfolding S3_def S4_def
+    by (simp add: conflict.simps)
+next
+  have "decide N S3 (trail_decide (state_trail S3) (Pos (Fun Q [b])), {}, None)"
+    unfolding S3_def state_trail_simp
+    using distinct_preds distinct_terms by (auto simp: trail_defined_lit_def intro: decideI)
+  hence "scl N S3 S4"
+    by (simp add: S3_def S4_def scl_def trail_decide_def)
+  moreover have "\<nexists>S. conflict N S4 S"
+  proof (rule notI, erule exE)
+    fix S
+    assume "conflict N S4 S"
+    thus False
+      unfolding S4_def
+      apply (cases rule: conflict.cases)
+      unfolding N_def Un_empty_right insert_iff
+      apply (elim disjE)
+      using distinct_preds
+      by (auto simp add: rename_clause_def clss_of_trail_def trail_false_cls_def
+          trail_false_lit_def subst_lit_def)
+  qed
+  ultimately show "reasonable_scl N S3 S4"
+    unfolding reasonable_scl_def by (simp add: S1_def)
+qed
+
+abbreviation renaming_vars5 where
+  "renaming_vars5 \<equiv> renaming_vars (\<Union> (vars_cls ` N))"
+
+definition S5 :: "('f, 'v) state" where
+  "S5 = ([
+    (Pos (Fun R [b]), Some ({#Neg (Fun Q [Var z]) \<cdot>l (Var o renaming_vars5)#},
+      Pos (Fun R [Var z]) \<cdot>l (Var o renaming_vars5), Var(renaming_vars5 z := b))),
+    (Pos (Fun Q [b]), None),
+    (Pos (Fun P [b]), None),
+    (Pos (Fun Q [a]), None),
+    (Pos (Fun P [a]), None)], {}, None)"
+
+lemma "regular_scl N S4 S5"
+proof (unfold regular_scl_def, rule disjI2, rule conjI)
+  show "\<not> conflict N S4 S5"
+    unfolding S4_def S5_def
+    by (simp add: conflict.simps)
+next
+  have "propagate N S4
+    (trail_propagate (state_trail S4) (Pos (Fun R [Var z]) \<cdot>l renaming_wrt N)
+      {#Neg (Fun Q [Var z]) \<cdot>l renaming_wrt N#} (Var(renaming_vars (\<Union> (vars_cls ` N)) z := b)),
+      {}, None)"
+    unfolding S4_def state_trail_simp
+    apply (rule propagateI[of "{#Neg (Fun Q [Var z]), Pos (Fun R [Var z])#}"])
+         apply (simp add: N_def)
+        apply (simp add: clss_of_trail_def rename_clause_def)
+       apply (auto simp add: subst_domain_def) []
+      apply (simp add: is_ground_cls_def subst_lit_def)
+     apply (simp add: trail_false_cls_def trail_false_lit_def subst_lit_def)
+    using distinct_preds distinct_terms
+    apply (auto simp add: trail_defined_lit_def subst_lit_def) []
+    done
+  hence "scl N S4 S5"
+    by (simp add: S4_def S5_def scl_def trail_propagate_def subst_lit_def)
+  moreover have "\<not> decide N S4 S5"
+    by (smt (verit, ccfv_SIG) S5_def decide.cases list.inject option.discI snd_conv state_trail_simp
+        trail_decide_def)
+  ultimately show "reasonable_scl N S4 S5"
+    unfolding reasonable_scl_def by simp
+qed
+
+abbreviation renaming_vars6 where
+  "renaming_vars6 \<equiv> renaming_vars (insert (renaming_vars (\<Union> (vars_cls ` N)) z) (\<Union> (vars_cls ` N)))"
+
+definition S6 :: "('f, 'v) state" where
+  "S6 = ([
+    (Pos (Fun S [b]), Some (
+      {#Neg (Fun R [Var w]) \<cdot>l (Var o renaming_vars6)#},
+      Pos (Fun S [Var w]) \<cdot>l (Var o renaming_vars6),
+      Var(renaming_vars6 w := b))),
+    (Pos (Fun R [b]), Some ({#Neg (Fun Q [Var z]) \<cdot>l (Var o renaming_vars5)#},
+      Pos (Fun R [Var z]) \<cdot>l (Var o renaming_vars5), Var(renaming_vars5 z := b))),
+    (Pos (Fun Q [b]), None),
+    (Pos (Fun P [b]), None),
+    (Pos (Fun Q [a]), None),
+    (Pos (Fun P [a]), None)], {}, None)"
+
+lemma state_trail_S6_conv: "state_trail S6 = trail_propagate (state_trail S5)
+  (Pos (Fun S [Var w]) \<cdot>l (Var o renaming_vars6))
+  {#Neg (Fun R [Var w]) \<cdot>l (Var o renaming_vars6)#}
+  (Var(renaming_vars6 w := b))"
+    by (simp add: S5_def S6_def N_def trail_propagate_def subst_lit_def)
+
+lemma "regular_scl N S5 S6"
+proof (unfold regular_scl_def, rule disjI2, rule conjI)
+  show "\<not> conflict N S5 S6"
+    unfolding S5_def S6_def
+    by (simp add: conflict.simps)
+next
+  have "propagate N S5 S6"
+    unfolding S5_def S6_def state_trail_S6_conv[unfolded S6_def state_trail_simp]
+    unfolding state_trail_simp
+    apply (rule propagateI[of "{#Neg (Fun R [Var w]), Pos (Fun S [Var w])#}"])
+         apply (simp add: N_def)
+        apply (simp add: clss_of_trail_def rename_clause_def)
+       apply (auto simp add: subst_domain_def) []
+      apply (simp add: is_ground_cls_def subst_lit_def)
+     apply (simp add: trail_false_cls_def trail_false_lit_def subst_lit_def)
+    using distinct_preds distinct_terms
+    apply (auto simp add: trail_defined_lit_def subst_lit_def) []
+    done
+  hence "scl N S5 S6"
+    by (simp add: scl_def)
+  moreover have "\<not> decide N S5 S6"
+    by (smt (verit, del_insts) Pair_inject S6_def decide.cases list.inject option.discI
+        trail_decide_def)
+  ultimately show "reasonable_scl N S5 S6"
+    unfolding reasonable_scl_def by simp
+qed
+
+abbreviation renaming_vars7 where
+  "renaming_vars7 \<equiv> renaming_vars {v, w, z, y, x,
+    renaming_vars {renaming_vars {v, w, z, y, x} z, v, w, z, y, x} w,
+    renaming_vars {v, w, z, y, x} z}"
+
+definition S7 :: "('f, 'v) state" where
+  "S7 = (state_trail S6, {}, Some (
+    {#Neg (Fun P [Var v]), Neg (Fun S [Var v])#} \<cdot> (Var o renaming_vars7),
+    Var(renaming_vars7 v := b)))"
+
+lemma "regular_scl N S6 S7"
+proof (unfold regular_scl_def, rule disjI1)
+  show "conflict N S6 S7"
+    unfolding S6_def S7_def
+    apply simp
+    apply (rule conflictI[of "{#Neg (Fun P [Var v]), Neg (Fun S [Var v])#}"])
+        apply (simp add: N_def)
+       apply (simp add: rename_clause_def clss_of_trail_def N_def)
+      apply (auto simp: subst_domain_def) []
+    using ground_b
+     apply (simp add: is_ground_cls_def subst_lit_def)
+    by (simp add: trail_false_cls_def trail_false_lit_def subst_lit_def)
+qed
+
+abbreviation renaming_wrt8 where
+  "renaming_wrt8 \<equiv> renaming_wrt
+    (N \<union> clss_of_trail (state_trail S6) \<union>
+      {{#Neg (Fun P [Var v]), Neg (Fun S [Var v])#} \<cdot> (Var \<circ> renaming_vars7)})"
+
+abbreviation mgu8 where
+  "mgu8 \<equiv> the (Unification.mgu
+    (atm_of (Pos (Fun S [Var w]) \<cdot>l (Var \<circ> renaming_vars6)))
+    (atm_of (Neg (Fun S [Var v]) \<cdot>l (Var \<circ> renaming_vars7))))"
+
+definition conflict8 where
+  "conflict8 = (
+    ({#Neg (Fun P [Var v])#} \<cdot> (Var \<circ> renaming_vars7) +
+     {#Neg (Fun R [Var w])#} \<cdot> (Var \<circ> renaming_vars6)) \<cdot> mgu8 \<cdot> renaming_wrt8,
+    restrict_subst
+      (vars_cls
+        (({#Neg (Fun P [Var v])#} \<cdot> (Var \<circ> renaming_vars7) +
+          {#Neg (Fun R [Var w])#} \<cdot> (Var \<circ> renaming_vars6)) \<cdot> mgu8 \<cdot> renaming_wrt8))
+      (inv_renaming' renaming_wrt8 \<odot> Var(renaming_vars7 v := b) \<odot> Var(renaming_vars6 w := b)))"
+
+definition S8 :: "('f, 'v) state" where
+  "S8 = (state_trail S6, {}, Some conflict8)"
+
+lemma "regular_scl N S7 S8"
+proof (unfold regular_scl_def, rule disjI2, rule conjI)
+  show "\<not> conflict N S7 S8"
+    unfolding S7_def by (simp add: conflict.simps)
+next
+  have "resolve N S7 S8"
+    unfolding S7_def S8_def conflict8_def resolve.simps
+    apply (rule exI[of _ "state_trail S6"])
+    apply (rule exI[of _ "tl (state_trail S6)"])
+    apply (rule exI[of _ "Pos (Fun S [Var w]) \<cdot>l (Var o renaming_vars6)"])
+    apply (rule exI[of _ "{#Neg (Fun R [Var w]) \<cdot>l (Var o renaming_vars6)#}"])
+    apply (rule exI[of _ "Var(renaming_vars6 w := b)"])
+    apply (rule exI[of _ "renaming_wrt
+        (N \<union> clss_of_trail (state_trail S6) \<union>
+         {{#Neg (Fun P [Var v])#} \<cdot> (Var \<circ> renaming_vars7) +
+          {#Neg (Fun S [Var v])#} \<cdot> (Var \<circ> renaming_vars7)})"])
+    apply (rule exI[of _ "{}"])
+    apply (rule exI[of _ "{#Neg (Fun P [Var v])#} \<cdot> (Var \<circ> renaming_vars7)"])
+    apply (rule exI[of _ "Neg (Fun S [Var v]) \<cdot>l (Var \<circ> renaming_vars7)"])
+    apply (rule exI[of _ "Var(renaming_vars7 v := b)"])
+    apply (rule exI[of _ "the (Unification.mgu
+          (atm_of
+            (Pos (Fun S [Var w]) \<cdot>l
+             (Var \<circ>
+              renaming_vars
+               (insert (renaming_vars (\<Union> (vars_cls ` N)) z)
+                 (\<Union> (vars_cls ` N))))))
+          (atm_of
+            (Neg (Fun S [Var v]) \<cdot>l (Var \<circ> renaming_vars7))))"])
+    unfolding prod.inject
+    apply (intro conjI)
+              apply simp_all
+       apply (simp add: S6_def subst_lit_def trail_propagate_def)
+    using distinct_preds apply (simp add: trail_level_cls_def subst_lit_def S6_def)
+    by (simp add: decompose_def zip_option.simps subst_list_def)
+  hence "scl N S7 S8"
+    unfolding scl_def by simp
+  moreover have "\<not> decide N S7 S8"
+    unfolding S7_def
+    by (simp add: decide.simps)
+  ultimately show "reasonable_scl N S7 S8"
+    unfolding reasonable_scl_def by simp
+qed
+
+definition S9 :: "('f, 'v) state" where
+  "S9 = (state_trail S5, {}, Some conflict8)"
+
+lemma tl_tail_propagate_def: "tl (trail_propagate \<Gamma> L C \<gamma>) = \<Gamma>"
+  by (simp add: trail_propagate_def)
+
+lemma "regular_scl N S8 S9"
+proof (unfold regular_scl_def, rule disjI2, rule conjI)
+  show "\<not> conflict N S8 S9"
+    unfolding S8_def by (simp add: conflict.simps)
+next
+  have "skip N S8 S9"
+    unfolding S5_def S8_def S9_def state_trail_S6_conv state_trail_simp
+    unfolding tl_tail_propagate_def
+    apply (rule skipI[of _ _ "fst conflict8" "snd conflict8", unfolded prod.collapse])
+    using distinct_preds
+    by (auto simp add: subst_lit_def conflict8_def decompose_def zip_option.simps N_def S6_def
+        clss_of_trail_def)
+  hence "scl N S8 S9"
+    unfolding scl_def by simp
+  moreover have "\<not> decide N S8 S9"
+    unfolding S8_def
+    by (simp add: decide.simps)
+  ultimately show "reasonable_scl N S8 S9"
+    unfolding reasonable_scl_def by simp
+qed
+
+definition conflict10 where
+  "conflict10 = conflict8"
+
+definition S10 :: "('f, 'v) state" where
+  "S10 = (state_trail S5, {}, Some conflict10)"
 
 end
 
