Simple_Clause_Learning/Correct_Termination.thy
@@ -4,7 +4,6 @@ begin
 
 context scl begin
 
-
 lemma assumes "(regular_scl N)\<^sup>*\<^sup>* initial_state S" and "conflict N S S'"
   shows "\<exists>C \<gamma>. state_conflict S' = Some (C, \<gamma>) \<and>
     (trail_level_cls (state_trail S) (C \<cdot> \<gamma>) = trail_level (state_trail S))"
@@ -160,101 +159,6 @@ proof (intro ballI allI impI)
   qed
 qed
 
-lemma trail_defined_lit_iff: "trail_defined_lit \<Gamma> L \<longleftrightarrow> atm_of L \<in> atm_of ` fst ` set \<Gamma>"
-  by (simp add: atm_of_in_atm_of_set_iff_in_set_or_uminus_in_set trail_defined_lit_def)
-
-lemma "trail_interp \<Gamma> \<subseteq> atm_of ` fst ` set \<Gamma>"
-  by (smt (verit, best) UN_iff image_iff insert_iff literal.case_eq_if singletonD subsetI trail_interp_def)
-
-lemma set_filter_insert_conv:
-  "{x \<in> insert y S. P x} = (if P y then insert y else id) {x \<in> S. P x}"
-  by auto
-
-lemma trail_interp_conv: "trail_interp \<Gamma> = atm_of ` {L \<in> fst ` set \<Gamma>. is_pos L}"
-proof (induction \<Gamma>)
-  case Nil
-  show ?case by (simp add: trail_interp_def)
-next
-  case (Cons Ln \<Gamma>)
-  then show ?case
-    unfolding list.set image_insert set_filter_insert_conv trail_interp_Cons'
-    by (simp add: literal.case_eq_if)
-qed
-
-lemma not_in_trail_interp_if_not_in_trail: "t \<notin> atm_of ` fst ` set \<Gamma> \<Longrightarrow> t \<notin> trail_interp \<Gamma>"
-  by (metis (no_types, lifting) atm_of_in_atm_of_set_iff_in_set_or_uminus_in_set
-      literal.sel(2) mem_Collect_eq trail_interp_conv)
-
-lemma trail_interp_lit_if_sound_and_trail_true:
-  shows "sound_trail N U \<Gamma> \<Longrightarrow> trail_true_lit \<Gamma> L \<Longrightarrow> trail_interp \<Gamma> \<TTurnstile>l L"
-proof (induction \<Gamma> rule: sound_trail.induct)
-  case Nil
-  thus ?case
-    by (simp add: trail_true_lit_def)
-next
-  case (Cons \<Gamma> K u)
-  show ?case
-  proof (cases "L = K \<or> L = - K")
-    case True
-    then show ?thesis 
-    proof (elim disjE)
-      assume "L = K"
-      thus ?thesis
-      proof (cases L; cases K)
-        fix t\<^sub>L t\<^sub>K
-        from \<open>L = K\<close> show "L = Pos t\<^sub>L \<Longrightarrow> K = Pos t\<^sub>K \<Longrightarrow> ?thesis"
-          by (simp add: trail_interp_def)
-      next
-        fix t\<^sub>L t\<^sub>K
-        from \<open>L = K\<close> show "L = Neg t\<^sub>L \<Longrightarrow> K = Neg t\<^sub>K \<Longrightarrow> ?thesis"
-          using Cons.hyps
-          by (simp add: trail_defined_lit_iff trail_interp_Cons'
-              not_in_trail_interp_if_not_in_trail)
-      qed simp_all
-    next
-      assume "L = - K"
-      then show ?thesis
-      proof (cases L; cases K)
-        fix t\<^sub>L t\<^sub>K
-        from \<open>L = - K\<close> show "L = Pos t\<^sub>L \<Longrightarrow> K = Neg t\<^sub>K \<Longrightarrow> ?thesis"
-          unfolding trail_interp_Cons'
-          using Cons.hyps(1) Cons.prems
-          by (metis (no_types, lifting) image_insert insertE list.simps(15) literal.distinct(1)
-              prod.sel(1) trail_defined_lit_def trail_true_lit_def)
-      next
-        fix t\<^sub>L t\<^sub>K
-        from \<open>L = - K\<close> show "L = Neg t\<^sub>L \<Longrightarrow> K = Pos t\<^sub>K \<Longrightarrow> ?thesis"
-          unfolding trail_interp_Cons'
-          using Cons.hyps(1) Cons.prems
-          by (metis (no_types, lifting) image_insert insertE list.simps(15) literal.distinct(1)
-              prod.sel(1) trail_defined_lit_def trail_true_lit_def)
-      qed simp_all
-    qed
-  next
-    case False
-    with Cons.prems have "trail_true_lit \<Gamma> L"
-      by (simp add: trail_true_lit_def)
-    with Cons.IH have "trail_interp \<Gamma> \<TTurnstile>l L"
-      by simp
-    with False show ?thesis
-      by (cases L; cases K) (simp_all add: trail_interp_def del: true_lit_iff)
-  qed
-qed
-
-lemma trail_interp_cls_if_sound_and_trail_true:
-  assumes "sound_trail N U \<Gamma>" and "trail_true_cls \<Gamma> C"
-  shows "trail_interp \<Gamma> \<TTurnstile> C"
-proof -
-  from \<open>trail_true_cls \<Gamma> C\<close> obtain L where "L \<in># C" and "trail_true_lit \<Gamma> L"
-    by (auto simp: trail_true_cls_def)
-  show ?thesis
-    unfolding true_cls_def
-  proof (rule bexI[OF _ \<open>L \<in># C\<close>])
-    show "trail_interp \<Gamma> \<TTurnstile>l L"
-      by (rule trail_interp_lit_if_sound_and_trail_true[OF \<open>sound_trail N U \<Gamma>\<close> \<open>trail_true_lit \<Gamma> L\<close>])
-  qed
-qed
-
 lemma set_removeAll_mset: "set_mset (removeAll_mset x M) = set_mset M - {x}"
   by simp
 
@@ -263,36 +167,6 @@ lemma trail_true_lit_Cons_iff: "trail_true_lit ((L, u) # \<Gamma>) K \<longleftr
 
 lemma trail_true_cls_Cons_iff: "trail_true_cls ((L, u) # \<Gamma>) C \<longleftrightarrow> L \<in># C \<or> trail_true_cls \<Gamma> C"
   by (auto simp: trail_true_cls_def trail_true_lit_Cons_iff)
-
-lemma trail_true_cls_iff_trail_interp_entails:
-  assumes "sound_trail N U \<Gamma>" "\<forall>L \<in># C. trail_defined_lit \<Gamma> L"
-  shows "trail_true_cls \<Gamma> C \<longleftrightarrow> trail_interp \<Gamma> \<TTurnstile> C"
-proof (rule iffI)
-  assume "trail_true_cls \<Gamma> C"
-  thus "trail_interp \<Gamma> \<TTurnstile> C"
-    using assms(1) trail_interp_cls_if_sound_and_trail_true by blast
-next
-  assume "trail_interp \<Gamma> \<TTurnstile> C"
-  then obtain L where "L \<in># C" and "trail_interp \<Gamma> \<TTurnstile>l L"
-    by (auto simp: true_cls_def)
-  show "trail_true_cls \<Gamma> C"
-  proof (cases L)
-    case (Pos t)
-    hence "t \<in> trail_interp \<Gamma>"
-      using \<open>trail_interp \<Gamma> \<TTurnstile>l L\<close> by simp
-    then show ?thesis
-      unfolding trail_true_cls_def
-      using \<open>L \<in># C\<close> Pos
-      by (metis assms(1) assms(2) trail_defined_lit_def trail_interp_lit_if_sound_and_trail_true
-          trail_true_lit_def true_lit_simps(2) uminus_Pos)
-  next
-    case (Neg t)
-    then show ?thesis
-      by (metis \<open>L \<in># C\<close> \<open>trail_interp \<Gamma> \<TTurnstile>l L\<close> assms(1) assms(2) trail_defined_lit_def
-          trail_interp_lit_if_sound_and_trail_true trail_true_cls_def trail_true_lit_def
-          true_lit_simps(1) true_lit_simps(2) uminus_Neg)
-  qed
-qed
 
 lemma trail_interp_clss_if_sound_and_trail_true:
   assumes "sound_trail N U \<Gamma>" and "trail_true_clss \<Gamma> CC"
